A12Kernel/Conformance.lean
@@ -79,6 +79,7 @@ import A12Kernel.Conformance.EnumerationElaboration
 import A12Kernel.Conformance.CheckedEnumeration
 import A12Kernel.Conformance.EnumerationValueList
 import A12Kernel.Conformance.EnumerationRepetitionNotUnique
+import A12Kernel.Conformance.FlatEnumeration
 import A12Kernel.Conformance.SemanticIndex
 import A12Kernel.Conformance.CustomCondition
 
